RAC of arithmetic properties: fix mini-c assign and substract semantic, update examples, more notations

Playground.v
@@ -13,6 +13,7 @@ Fact ir5 : Int.inRange 5. now split. Qed.
 Fact ir10 : Int.inRange 10 . now split. Qed.
 Fact ir14 : Int.inRange 14. now split. Qed.
 Fact ir15 : Int.inRange 15. now split. Qed.
+Definition two := Int (Int.mkMI 2 ir2).
 Definition three := Int (Int.mkMI 3 ir3).
 Definition five := Int (Int.mkMI 5 ir5).
 Definition ten := Int (Int.mkMI 10 ir10).
@@ -21,39 +22,34 @@ Definition funs := ⊥{"test"\("a" :: "b" :: nil, <{ return ("b") }>)}.
 
 
 Example stmt_test :
-    forall o m,     
-    let v := fst o in 
-    let l := snd o in 
-    c_stmt_sem
-    o m 
-
+    forall v l m,     
+    
+    [(v{"g"\UInt,"z"\UInt,"x"\UInt,"y"\UInt,"out"\UInt},l)  ~ m ]
+    |=
     <{
     "x" = 5 ;
     "y" = 10;
     "z" = "x" + "y";
     "g" = 0;
-    "out" <-  (1+2, ("x"+"g")) "test";
+    "out" <- (1+2,"x"+"g") "test";
 
     if ("z" <= 14)
         "g" = "z"
     else 
         "g" = "out" / 5
     }>
-    
-    (v{"g"\ one, "out"\five, "g"\ zero, "z"\ fifteen, "y"\ ten, "x" \ five}, l) m
+    =>
+    [ (v{"g"\ one, "out"\five, "g"\ zero, "z"\ fifteen, "y"\ ten, "x" \ five,"g"\UInt,"z"\UInt,"x"\UInt,"y"\UInt,"out"\UInt}, l) ~ m]
    .
 Proof.
-    intros. 
-     apply S_Seq with (v{"x" \ five},l) m.
-     apply S_Assign. apply C_E_Int.
-     apply S_Seq with (v{"y"\ten,"x"\five}, l) m.
-     - apply S_Assign. apply C_E_Int.
-     - apply S_Seq with (v{"z" \ fifteen, "y" \ ten, "x" \ five}, l) m.
-        + apply S_Assign. apply C_E_BinOpInt with (z:=5) (z':=10) (z_ir:=ir5) (z'_ir:=ir10) ; 
+    intros. eapply S_Seq. fstassgn. apply C_E_Int. eapply S_Seq.
+     - fstassgn. apply C_E_Int.
+     - eapply S_Seq.
+        + fstassgn. apply C_E_BinOpInt with (z:=5) (z':=10) (z_ir:=ir5) (z'_ir:=ir10) ; 
           now apply C_E_Var. 
-        + apply S_Seq  with (v{"g"\ zero, "z" \ fifteen, "y" \ ten, "x" \ five}, l) m. 
-          ++ apply S_Assign. apply C_E_Int.
-          ++ apply S_Seq with (v{"out"\five, "g"\ zero, "z" \ fifteen, "y" \ ten, "x" \ five}, l) m.
+        + eapply S_Seq.
+          ++ fstassgn. apply C_E_Int.
+          ++ eapply S_Seq.
           {  
           apply S_FCall with
               (resf:="out")
@@ -66,9 +62,9 @@ Proof.
             .
             - reflexivity.
             - simpl. constructor. 
-                apply C_E_BinOpInt with  (z:=1) (z':=2) (z_ir:=oneinRange) (z'_ir:=ir2) ; now constructor.
+                apply C_E_BinOpInt with (z_ir:=oneinRange) (z'_ir:=ir2) ; now constructor.
                 constructor.
-                apply C_E_BinOpInt with  (z:=5) (z':=0) (z_ir:=ir5) (z'_ir:=zeroinRange) ; now constructor.
+                apply C_E_BinOpInt with (z_ir:=ir5) (z'_ir:=zeroinRange) ; now constructor.
                 constructor.
             - simpl. constructor. now constructor.
             - simpl. constructor.
@@ -77,11 +73,41 @@ Proof.
             * apply C_E_BinOpFalse with 15 14 ir15 ir14 ; try now constructor.
             simpl. intro H. destruct H. reflexivity.
             * reflexivity.
-            * apply S_Assign. apply C_E_BinOpInt with  (z:=(5)) (z':=5) (z_ir:=ir5) (z'_ir:=ir5) ; now constructor.
+            * reassign (Int.mkMI 0 zeroinRange). apply C_E_BinOpInt with  (z:=(5)) (z':=5) (z_ir:=ir5) (z'_ir:=ir5) ; now constructor.
 Qed.
-
-
-Close Scope mini_c_scope.
 
 Example test_dom : ~ dom (fun x => if x>?2 then Some (x*2) else None) 2.
 Proof. intro contra. inversion contra. discriminate. Qed.
+
+
+Example whileex : [(⊥{"m"\zero, "n"\three},⊥) ~ ⊥] |= <{ while  "n" > 0  <{"n" = "n" - 1 ; "m" = "m" + 1}> }> => [(⊥{"m"\three, "n"\zero,"m"\two, "n"\one,"m"\one, "n"\two,"m"\zero, "n"\three},⊥) ~ ⊥].
+Proof.
+    apply S_While. apply S_IfTrue with one.
+    - apply C_E_BinOpTrue with 3 0 ir3 zeroinRange. apply C_E_Var. reflexivity. apply C_E_Int. reflexivity.
+    - intro contra. inversion contra. 
+    - { eapply S_Seq.  eapply S_Seq.
+        - reassign (Int.mkMI 3 ir3).  apply C_E_BinOpInt with  (z_ir := ir3) (z'_ir := oneinRange).  apply C_E_Var. reflexivity. apply C_E_Int.
+        - reassign (Int.mkMI 0 zeroinRange). apply C_E_BinOpInt with (z_ir := zeroinRange) (z'_ir := oneinRange). apply C_E_Var. reflexivity. apply C_E_Int.
+        -  apply S_While. eapply S_IfTrue.
+           apply C_E_BinOpTrue with (z_ir:=ir2) (z'_ir:=zeroinRange). apply C_E_Var. reflexivity. apply C_E_Int. reflexivity.
+            intro contra. inversion contra.
+            {
+                eapply S_Seq. eapply S_Seq.
+                - reassign (Int.mkMI 2 ir2).  apply C_E_BinOpInt with (z_ir := ir2) (z'_ir := oneinRange). apply C_E_Var. reflexivity. apply C_E_Int.
+                - reassign (Int.mkMI 1 oneinRange). apply C_E_BinOpInt with (z_ir := oneinRange) (z'_ir := oneinRange). apply C_E_Var. reflexivity. apply C_E_Int.
+                - apply S_While. eapply S_IfTrue.
+                apply C_E_BinOpTrue with (z_ir:=oneinRange) (z'_ir:=zeroinRange). apply C_E_Var. reflexivity. apply C_E_Int. reflexivity.
+                 intro contra. inversion contra.
+                 {
+                     eapply S_Seq. eapply S_Seq.
+                     - reassign (Int.mkMI 1 oneinRange).  apply C_E_BinOpInt with (z_ir := oneinRange) (z'_ir := oneinRange). simpl. apply C_E_Var. reflexivity. apply C_E_Int.
+                     - reassign (Int.mkMI 2 ir2). apply C_E_BinOpInt with (z_ir:=ir2) (z'_ir:=oneinRange). apply C_E_Var. reflexivity. apply C_E_Int.
+                     - apply S_While. eapply S_IfFalse.
+                     apply C_E_BinOpFalse with (z_ir:=zeroinRange) (z'_ir:=zeroinRange). apply C_E_Var. reflexivity. apply C_E_Int. intro contra. inversion contra. reflexivity.                   
+                    apply S_skip. 
+                
+                }
+           
+           }
+     }
+Qed.
