Semantics.v
@@ -3,98 +3,99 @@ Require Import RAC.Notations.
 Require Import RAC.Utils.
 Require Import ZArith.ZArith.
 From Coq Require Import Strings.String.
-Open Scope mini_c_scope.
 
+
+Open Scope mini_c_scope.
+Declare Scope mini_c_exp_scope.
 
 Inductive c_exp_sem (env : Ω) : c_exp -> Value -> Prop :=
-| C_E_Int (z:Z) in_range: env ⊨ z => (Int.mkMI z in_range)
+| C_E_Int (z:Z) in_range: env |= z => (Int.mkMI z in_range)
 | C_E_Var (x:V) z  : 
     (fst env)(x:string) = Some (Int z) -> 
-    env ⊨ x => z
+    env |= x => z
 | C_E_BinOpInt e e' (z z':Z) op z_ir z'_ir 
     (H:Int.inRange (⋄ op z z')) :
-    env ⊨ e =>  (Int.mkMI z z_ir) ->
-    env ⊨ e' =>  (Int.mkMI z' z'_ir) ->
-    env ⊨ BinOpInt e op e' => Int.mkMI ((⋄ op) z z') H
+    env |= e =>  (Int.mkMI z z_ir) ->
+    env |= e' =>  (Int.mkMI z' z'_ir) ->
+    env |= BinOpInt e op e' => Int.mkMI ((⋄ op) z z') H
 | C_E_BinOpTrue e e' (z z' : Z) z_ir z'_ir op :
-    env ⊨ e => (Int.mkMI z z_ir) ->
-    env ⊨ e' => (Int.mkMI z z'_ir) ->
+    env |= e => (Int.mkMI z z_ir) ->
+    env |= e' => (Int.mkMI z' z'_ir) ->
     ((◁ op) z z' -> True) ->
-    env ⊨ BinOpBool e op e' => one
+    env |= BinOpBool e op e' => one
 | C_E_BinOpFalse e e' (z z' : Z) op z_ir z'_ir :
-    env ⊨ e => (Int.mkMI z z_ir) -> 
-    env ⊨ e' => (Int.mkMI z' z'_ir) -> 
+    env |= e => (Int.mkMI z z_ir) -> 
+    env |= e' => (Int.mkMI z' z'_ir) -> 
     ((◁ op) z z' -> False) ->
-    env ⊨ BinOpBool e op e' => zero
+    env |= BinOpBool e op e' => zero
 
-where  "Ω '⊨' e => v" := (c_exp_sem Ω e v).
+where  "Ω '|=' e => v" := (c_exp_sem Ω e v) : mini_c_exp_scope.
 
+Declare Scope mini_c_decl_scope.
+Definition c_decl_sem (env env':Ω) (mem mem':M) d : Prop := 
+        forall t x u,
+        (fst env) x  = None -> 
+        (u = UInt \/ u = UMpz ) ->
+        d = C_Decl t x -> env' = ((fst env){x\u},snd env) /\ mem = mem'
+        .
+Notation " [ Ω ~ M ]  |= d => [ Ω' ~ M' ]" := (c_decl_sem Ω M d Ω' M') : mini_c_decl_scope.
 
-Inductive c_decl_sem (env:Ω) (mem:M) : c_decl -> Ω -> M -> Prop := 
-    | Decl t x (u:Value) : 
-        (* v x = ⊥ -> (env,mem ⊨ C_Decl t x => (v{x\u},l),mem) *)
-        c_decl_sem  env mem (C_Decl t x) ((fst env){x\u}, snd env) mem 
-  (* where 
-  "Ω ',' M '⊨' d '=>' Ω' ',' M'" := (c_decl_sem d Ω M Ω' M')  *)
-.
-
-
+Open Scope mini_c_exp_scope.
+Declare Scope mini_c_stmt_scope.
 Inductive c_stmt_sem (env:Ω) (mem:M) : S -> Ω -> M -> Prop := 
-    | S_skip  : c_stmt_sem env mem <{ skip }> env mem
-    | S_Assign x z e : 
-        (* in v x Int + Uint  *)
-        env ⊨ e => z ->
-        c_stmt_sem  env mem <{x = e}> ((fst env){x\z},snd env) mem
+    | S_skip  :  [ env ~ mem ] |= <{ skip }> => [env ~ mem]
+    | S_Assign x z e: 
+        (exists n, (fst env) x = Some (Int n)) \/  (fst env) x = Some UInt ->
+        env |= e => z ->
+        [env~mem] |= <{x = e}> => [((fst env){x\z},snd env) ~  mem]
     | S_IfTrue env' mem' z e s s' :
-        env ⊨ e => z ->
+        env |= e => z ->
         z <>  Int.mkMI 0 zeroinRange ->
-        c_stmt_sem env mem s  env' mem' ->
-        c_stmt_sem  env mem <{ if (e) s else s'}> env' mem' 
+        [env~mem ] |= s => [ env' ~ mem'] ->
+        [ env ~ mem ] |= <{ if e s else s'}> => [ env' ~ mem' ]
     | S_IfFalse env' mem' z e s s' :
-        env ⊨ e => z ->
+        env |= e => z ->
         z = Int.mkMI 0 zeroinRange ->
-        c_stmt_sem  env mem s' env' mem' ->
-        c_stmt_sem  env mem <{ if (e) s else s' }> env' mem' 
+        [ env ~ mem] |= s' => [ env' ~ mem'] ->
+        [ env ~ mem ] |= <{ if e s else s'}> => [ env' ~ mem' ]
     | S_While e s   env' mem' :
-        c_stmt_sem  env mem (If e (Seq s (While e s)) Skip) env' mem' ->
-        c_stmt_sem  env mem <{ while (e) s }> env' mem' 
+        [ env ~ mem] |= <{ if e s ; while e s else skip }> => [ env' ~ mem' ] ->
+        [ env ~ mem] |= <{ while e s }> => [ env' ~ mem' ]
     | S_Seq  env' mem' env'' mem'' s s' :
-        c_stmt_sem  env mem s env' mem' -> 
-        c_stmt_sem  env' mem' s' env'' mem'' ->
-        c_stmt_sem env mem <{ s ; s' }>  env'' mem''
+    [ env ~ mem] |= s => [ env' ~ mem'] ->
+    [ env' ~ mem'] |= s' => [ env'' ~ mem''] ->
+    [ env ~ mem] |= <{ s ; s' }> =>  [ env'' ~ mem''] 
 
     | S_FCall (funs:F) f b env' mem' c xargs eargs zargs resf z  : 
         let eToz := List.combine eargs zargs in
         let xToz := List.combine xargs zargs in
         funs f = Some (xargs,b) ->
-        List.Forall (fun p => p) (List.map (fun ez => env ⊨ (fst ez) => (snd ez)) eToz)  ->
-        c_stmt_sem ((p_map_addall ⊥ xToz),⊥) mem b env' mem' ->
+        List.Forall (fun p => p) (List.map (fun ez => env |= (fst ez) => (snd ez)) eToz)  ->
+         [((p_map_addall ⊥ xToz),⊥)  ~ mem] |= b => [env' ~ mem'] ->
         (fst env') resf = Some z ->
-        
-        c_stmt_sem env mem (FCall c f eargs) ((fst env){c\z},(snd env)) mem'
+        [ env ~ mem ] |= (FCall c f eargs) => [((fst env){c\z},(snd env)) ~ mem']
 
     | S_PCall (procs:P) p b env' mem' xargs eargs zargs  : 
         let eToz := List.combine eargs zargs in
         let xToz := List.combine xargs zargs in
         procs p = Some (xargs,b) ->
-        List.Forall (fun p => p) (List.map (fun ez => env ⊨ (fst ez) => (snd ez)) eToz)  ->
-        c_stmt_sem ((p_map_addall ⊥ xToz),⊥) mem b env' mem' ->
-        
-        c_stmt_sem env mem (PCall p eargs) env mem'
+        List.Forall (fun p => p) (List.map (fun ez => env |= (fst ez) => (snd ez)) eToz)  ->
+        [ ((p_map_addall ⊥ xToz),⊥) ~ mem] |= b => [env' ~ mem'] ->
+        [ env ~ mem ] |= PCall p eargs => [ env ~ mem' ]
 
     | S_Return e z resf : 
-         env ⊨ e => z -> c_stmt_sem env mem <{ return(e) }> ((fst env){resf\z},snd env) mem
+         env |= e => z -> [env ~ mem] |= <{ return e }> =>  [((fst env){resf\z},snd env) ~ mem]
 
     | S_PAssert  e z :
-        env ⊨ e => z -> z <>  zero ->
-        c_stmt_sem env mem <{ assert (e) }> env mem
+        env |= e => z -> z <>  zero ->
+        [env ~ mem] |= <{ assert e }> => [env ~ mem] 
 
     (* | S_LAssert p :
-        env ⊨ p => one -> (* must be fsl *)
+        env |= p => one -> (* must be fsl *)
         c_stmt_sem env mem <{ /*@ assert p */ }> env mem *)
 
- (* where "Ω ',' M '⊨' s '=>' Ω' ',' M'" := (c_stmt_sem s Ω M Ω' M') *)
-    .
+        where " [ Ω  ~ M ]  |= s => [ Ω' ~ M' ] "  := (c_stmt_sem Ω M s Ω' M')
+        .
 
 
 
@@ -113,16 +114,20 @@ Inductive fsl_term_sem (env:Ω) : LT -> Value -> Prop :=
     fsl_term_sem env (T_BinOp t op t') ((fsl_binop_int_model op) zint z'int) *)
 .
 
-
 (* Inductive fsl_pred_sem : B -> Ω -> M -> Ω -> M -> Prop :=
 | none
 . *)
 
 (* 
 Inductive fsl_assert_sem : S -> Ω -> M -> Ω -> M -> Prop := 
-| P_Assert env mem p :  env ⊨ p => mkMI 1 oneinRange -> 
+| P_Assert env mem p :  env |= p => mkMI 1 oneinRange -> 
     fsl_assert_sem (LAssert p) env mem env mem
 . *)
 
 
 (* todo GMP semantics *)
+
+
+
+Ltac fstassgn := apply S_Assign ; [now right|idtac] . 
+Ltac reassign n := apply S_Assign ; [ now left ; now exists n| idtac]. 
